towards using set_eq for justifications

theories/LightStates/messages.v
@@ -20,14 +20,20 @@ Parameter Hash : message -> hash.
 
 Parameter hash_injective : Injective Hash.
 
-Lemma message_eq_dec : forall (msg1 msg2 : message), {msg1 = msg2} + {msg1 <> msg2}.
+Definition message_eq (msg1 msg2 : message) : Prop :=
+  match msg1, msg2 with 
+    (c1, v1, j1), (c2, v2,j2) => 
+      c1 = c2 /\ v1 = v2 /\ justification_eq j1 j2
+  end.
+
+Lemma message_eq_dec : forall (msg1 msg2 : message), {message_eq msg1 msg2} + {~ message_eq msg1 msg2}.
 Proof.
   destruct msg1 as [(c1, v1) j1]. destruct msg2 as [(c2, v2) j2].
   destruct (c_eq_dec c1 c2).
   - subst. destruct (v_eq_dec v1 v2).
     + subst. destruct (justification_eq_dec j1 j2).
-      * subst. left. reflexivity.
-      * right. intro. inversion H; subst. apply n. reflexivity.
-    + right. intro. inversion H; subst. apply n. reflexivity.
+      * left. simpl. split; try reflexivity. split; try reflexivity. assumption.
+      * right. intro. simpl in H. destruct H as [_ [_ Heq]]. apply n. assumption.
+    + right. intro.  simpl in H. destruct H as [_ [Heq _]]; subst. apply n. reflexivity.
   - right. intro. inversion H; subst. apply n. reflexivity.
 Qed.
