theories/LightStates/hashes.v
@@ -17,7 +17,4 @@ Definition justification_in := set_mem hash_eq_dec.
 
 Definition justification_eq := @set_eq hash.
 
-Lemma justification_eq_dec : forall (hs1 hs2 : justification), {hs1 = hs2} + {hs1 <> hs2}.
-Proof.
-  intros. apply list_eq_dec. apply hash_eq_dec.
-Qed.
+Definition justification_eq_dec := set_eq_dec hash_eq_dec.
